bin/output/main_double_0.dfy
@@ -2,99 +2,100 @@
 include "utils.dfy"
 
 /******************************* UDTS ***************************************/
-class Sum{
+class StatsUtilList{
+	var period: int;
 }
 class CasperDataRecord{
-	var v1: int;
-	var v2: int;
+	var x: int;
+	var y: int;
 }
 
 
 /***************************** DO MAP ***************************************/
 
-function emit0(casper_data_set: seq<CasperDataRecord>, i0: int, i: int, loop0: bool) : seq<(int, int)>
+function emit0(casper_data_set: seq<CasperDataRecord>, i0: int, i: int, yVariance: int, xVariance: int, loop0: bool) : seq<(int, int)>
 	requires null !in casper_data_set
 	reads casper_data_set
 	requires 0 <= i < |casper_data_set|
-	ensures emit0(casper_data_set, i0, i, loop0) == [(1,(casper_data_set[i].v1-casper_data_set[i].v2)*(casper_data_set[i].v1-casper_data_set[i].v2))]
+	ensures emit0(casper_data_set, i0, i, yVariance, xVariance, loop0) == [(1,(casper_data_set[i].x-xVariance)*(casper_data_set[i].y-yVariance))]
 {
-	[(1,(casper_data_set[i].v1-casper_data_set[i].v2)*(casper_data_set[i].v1-casper_data_set[i].v2))]
+	[(1,(casper_data_set[i].x-xVariance)*(casper_data_set[i].y-yVariance))]
 }
 
 
-function domap (casper_data_set: seq<CasperDataRecord>, i0: int, i: int, loop0: bool) : seq<(int, int)>
+function domap (casper_data_set: seq<CasperDataRecord>, i0: int, i: int, yVariance: int, xVariance: int, loop0: bool) : seq<(int, int)>
     requires null !in casper_data_set
 	reads casper_data_set
 	requires 0 <= i < |casper_data_set|
-    ensures domap(casper_data_set, i0, i, loop0) == emit0(casper_data_set, i0, i, loop0)
+    ensures domap(casper_data_set, i0, i, yVariance, xVariance, loop0) == emit0(casper_data_set, i0, i, yVariance, xVariance, loop0)
 {
-    emit0(casper_data_set, i0, i, loop0)
+    emit0(casper_data_set, i0, i, yVariance, xVariance, loop0)
 }
 
 /***************************** MAPPER ***************************************/
 
-function mapper (casper_data_set: seq<CasperDataRecord>, i0: int, i: int, loop0: bool) : seq<(int, int)>
+function mapper (casper_data_set: seq<CasperDataRecord>, i0: int, i: int, yVariance: int, xVariance: int, loop0: bool) : seq<(int, int)>
     requires null !in casper_data_set
 	reads casper_data_set
 	requires 0 <= i <= |casper_data_set|
 {
     if i == 0 then []
-    else domap(casper_data_set, i0, i-1, loop0) + mapper(casper_data_set, i0, i-1, loop0)
+    else domap(casper_data_set, i0, i-1, yVariance, xVariance, loop0) + mapper(casper_data_set, i0, i-1, yVariance, xVariance, loop0)
 }
 
 /***************************** DO REDUCE ************************************/
 
-function doreduce(input: seq<(int, int)>, key: int, loop0: bool) : int
+function doreduce(input: seq<(int, int)>, key: int, yVariance: int, xVariance: int, loop0: bool) : int
     ensures (|input| > 0 && input[0].0 == key) ==> 
-        doreduce(input, key, loop0) == (if key == 1 then ((input[0].1+doreduce(input[1..], key, loop0))) else ((input[0].1+doreduce(input[1..], key, loop0))))
+        doreduce(input, key, yVariance, xVariance, loop0) == (if key == 1 then ((input[0].1+doreduce(input[1..], key, yVariance, xVariance, loop0))) else ((input[0].1+doreduce(input[1..], key, yVariance, xVariance, loop0))))
     ensures (|input| > 0 && input[0].0 != key) ==> 
-        doreduce(input, key, loop0) == doreduce(input[1..], key, loop0)
+        doreduce(input, key, yVariance, xVariance, loop0) == doreduce(input[1..], key, yVariance, xVariance, loop0)
 {
     if input == [] then (if key == 1 then 0 else 0 )
-    else if input[0].0 == key then (if key == 1 then ((input[0].1+doreduce(input[1..], key, loop0))) else ((input[0].1+doreduce(input[1..], key, loop0))))
-    else doreduce(input[1..], key, loop0)
+    else if input[0].0 == key then (if key == 1 then ((input[0].1+doreduce(input[1..], key, yVariance, xVariance, loop0))) else ((input[0].1+doreduce(input[1..], key, yVariance, xVariance, loop0))))
+    else doreduce(input[1..], key, yVariance, xVariance, loop0)
 }
 
 /******************************* HARNESS ************************************/    
 
-predicate loopInvariant (casper_data_set: seq<CasperDataRecord>, dist: int, dist0: int, i: int, i0: int, loop0: bool)
+predicate loopInvariant (casper_data_set: seq<CasperDataRecord>, covariance: int, covariance0: int, i: int, i0: int, yVariance: int, xVariance: int, loop0: bool)
     requires null !in casper_data_set
 	reads casper_data_set
 	
 {
     0 <= i <= |casper_data_set| &&
-	(dist == (doreduce(mapper(casper_data_set,i0,i,loop0),1, loop0)))
+	(covariance == (doreduce(mapper(casper_data_set,i0,i,yVariance,xVariance,loop0),1, yVariance, xVariance, loop0)))
 }
 
-predicate postCondition (casper_data_set: seq<CasperDataRecord>, dist: int, dist0: int, i: int, i0: int, loop0: bool)
+predicate postCondition (casper_data_set: seq<CasperDataRecord>, covariance: int, covariance0: int, i: int, i0: int, yVariance: int, xVariance: int, loop0: bool)
     requires null !in casper_data_set
 	reads casper_data_set
 	
 {
     i == |casper_data_set| &&
-	(dist == (doreduce(mapper(casper_data_set,i0,i,loop0),1, loop0)))
+	(covariance == (doreduce(mapper(casper_data_set,i0,i,yVariance,xVariance,loop0),1, yVariance, xVariance, loop0)))
 }
 
-method harness (casper_data_set: seq<CasperDataRecord>, dist: int, i: int)
+method harness (casper_data_set: seq<CasperDataRecord>, covariance: int, yVariance: int, xVariance: int, i: int)
     requires null !in casper_data_set
 {
-    var dist0 := 0;
+    var covariance0 := 0;
 	var loop0 := false;
 	var i0 := 0;
 	
-    assert loopInvariant(casper_data_set,dist0,0,i0,0,loop0);
+    assert loopInvariant(casper_data_set,covariance0,0,i0,0,yVariance,xVariance,loop0);
 
-	if(loopInvariant(casper_data_set,dist,0,i,0,loop0) && (i<|casper_data_set|))
+	if(loopInvariant(casper_data_set,covariance,0,i,0,yVariance,xVariance,loop0) && (i<|casper_data_set|))
 	{
+		var ind_covariance := covariance;
+		ind_covariance := (covariance+((casper_data_set[i].x-xVariance)*(casper_data_set[i].y-yVariance)));
 		var ind_i := i;
 		ind_i := (i+1);
-		var ind_dist := dist;
-		ind_dist := (dist+((casper_data_set[i].v1-casper_data_set[i].v2)*(casper_data_set[i].v1-casper_data_set[i].v2)));
-		assert loopInvariant(casper_data_set,ind_dist,dist0,ind_i,i0,loop0);
+		assert loopInvariant(casper_data_set,ind_covariance,covariance0,ind_i,i0,yVariance,xVariance,loop0);
 	}
 
-	if(loopInvariant(casper_data_set,dist,0,i,0,loop0) && !(i<|casper_data_set|))
+	if(loopInvariant(casper_data_set,covariance,0,i,0,yVariance,xVariance,loop0) && !(i<|casper_data_set|))
 	{
-		assert postCondition(casper_data_set,dist,0,i,0,loop0);
+		assert postCondition(casper_data_set,covariance,0,i,0,yVariance,xVariance,loop0);
 	}
 }
