bin/output/main_double_0_CSG.dfy
@@ -2,33 +2,34 @@
 include "utils.dfy"
 
 /******************************* UDTS ***************************************/
-class Sum{
+class StatsUtilList{
+	var period: int;
 }
 class CasperDataRecord{
-	var v1: int;
-	var v2: int;
+	var x: int;
+	var y: int;
 }
 
 
 /******************************* HARNESS ************************************/  
-function doreduce(input: seq<(int, int)>, key: int, loop0: bool) : int
+function doreduce(input: seq<(int, int)>, key: int, yVariance: int, xVariance: int, loop0: bool) : int
     ensures (|input| > 0 && input[0].0 == key) ==> 
-        doreduce(input, key, loop0) == (if key == 1 then ((input[0].1+doreduce(input[1..], key, loop0))) else ((input[0].1+doreduce(input[1..], key, loop0))))
+        doreduce(input, key, yVariance, xVariance, loop0) == (if key == 1 then ((input[0].1+doreduce(input[1..], key, yVariance, xVariance, loop0))) else ((input[0].1+doreduce(input[1..], key, yVariance, xVariance, loop0))))
     ensures (|input| > 0 && input[0].0 != key) ==> 
-        doreduce(input, key, loop0) == doreduce(input[1..], key, loop0)
+        doreduce(input, key, yVariance, xVariance, loop0) == doreduce(input[1..], key, yVariance, xVariance, loop0)
 {
     if input == [] then (if key == 1 then 0 else 0 )
-    else if input[0].0 == key then (if key == 1 then ((input[0].1+doreduce(input[1..], key, loop0))) else ((input[0].1+doreduce(input[1..], key, loop0))))
-    else doreduce(input[1..], key, loop0)
+    else if input[0].0 == key then (if key == 1 then ((input[0].1+doreduce(input[1..], key, yVariance, xVariance, loop0))) else ((input[0].1+doreduce(input[1..], key, yVariance, xVariance, loop0))))
+    else doreduce(input[1..], key, yVariance, xVariance, loop0)
 }  
 
-lemma LemmaCSG_dist (a: seq<(int, int)>, b: seq<(int, int)>, key: int, loop0: bool)
+lemma LemmaCSG_covariance (a: seq<(int, int)>, b: seq<(int, int)>, key: int, yVariance: int, xVariance: int, loop0: bool)
 	requires key == 1
-ensures doreduce(a+b, key, loop0) == ((doreduce(b, key, loop0)+doreduce(a, key, loop0)))
+ensures doreduce(a+b, key, yVariance, xVariance, loop0) == ((doreduce(b, key, yVariance, xVariance, loop0)+doreduce(a, key, yVariance, xVariance, loop0)))
 {
 	if a != []
 	{
-		LemmaCSG_dist(a[1..], b, key, loop0);
+		LemmaCSG_covariance(a[1..], b, key, yVariance, xVariance, loop0);
 		assert a + b == [a[0]] + (a[1..] + b);
 	}
 }
